refactored bloomfilter proofs such that all non-probabilistic statements are provided in the structure definition

Structures/BloomFilter.v
@@ -12,7 +12,7 @@ Unset Strict Implicit.
 Unset Printing Implicit Defensive.
 
 From BloomFilter
-     Require Import Parameters Hash HashVec Comp Notationv1 BitVector FixedList.
+     Require Import Parameters Hash HashVec Comp Notationv1 BitVector FixedList InvMisc.
 
 
 
@@ -38,8 +38,8 @@ Section BloomFilter.
 
 
 
-    Record BloomFilter := mkBloomFilter {
-                              bloomfilter_state: BitVector
+  Record BloomFilter := mkBloomFilter {
+                            bloomfilter_state: BitVector
                           }.
 
   Definition BloomFilter_prod (bf: BloomFilter) :=
@@ -78,7 +78,7 @@ Section BloomFilter.
       (set_tnth (bloomfilter_state bf) true value).
 
   Definition bloomfilter_get_bit (value: 'I_(Hash_size.+1)) bf : bool :=
-      (tnth (bloomfilter_state bf) value).
+    (tnth (bloomfilter_state bf) value).
 
   Fixpoint bloomfilter_add_internal (items: seq 'I_(Hash_size.+1)) bf : BloomFilter :=
     match items with
@@ -101,4 +101,178 @@ Section BloomFilter.
       let qres := bloomfilter_query_internal (tval hash_vec) bf in
       ret (new_hashes, qres).
 
+
+  Definition bloomfilter_add_multiple  hsh_0 bf_0 values :=
+    @foldr B (Comp [finType of k.-tuple (HashState n) * BloomFilter])
+           (fun val hsh_bf =>
+              res_1 <-$ hsh_bf;
+                let (hsh, bf) := res_1 in
+                bloomfilter_add val hsh bf) (ret (hsh_0, bf_0)) values.
+
+  
+
+  Definition bloomfilter_new : BloomFilter.
+    apply mkBloomFilter.
+    apply Tuple with (nseq Hash_size.+1 false).
+      by rewrite size_nseq.
+  Defined.
+
+
+  
+
+  Lemma bloomfilter_new_empty_bits b : ~~ bloomfilter_get_bit b bloomfilter_new .
+  Proof.
+    clear k n Hkgt0.
+    rewrite/bloomfilter_get_bit/bloomfilter_new //=.
+    elim: Hash_size b => [[[|//=] Hm]|//= n IHn] //=.
+    move=> [[| b] Hb]; rewrite /tnth //=.
+    move: (Hb); move/ltn_SnnP: Hb => Hb' Hb;move: (IHn (Ordinal Hb'));rewrite /tnth //=.
+    clear.
+
+    move: (size_nseq n.+1 _)  => Hprf.
+    move:(tnth_default _ _) (tnth_default _ _); clear Hb => b1 b2.
+
+    have ->: (false :: nseq n false) = (nseq n.+1 false); first by [].
+    move: Hb'; rewrite -Hprf; clear Hprf.
+    move: (n.+1); clear n; elim: b => [//= n'|]; first by case: (nseq n' _).
+    move=>  b IHb.
+    case => [//=| n].
+      by move=>//=/ltn_SnnP/(IHb n) IHb' H; apply IHb'.
+  Qed.
+
+  Lemma bloomfilter_new_empty bs : length bs > 0 -> ~~ bloomfilter_query_internal bs bloomfilter_new .
+  Proof.
+    clear k n Hkgt0.
+    case: bs => [//=| b1 [//=| b2 bs]] Hlen; first by rewrite Bool.andb_true_r; apply bloomfilter_new_empty_bits.
+    rewrite Bool.negb_andb; apply/orP; left; apply bloomfilter_new_empty_bits.
+  Qed.
+
+  
+  
+  Lemma bloomfilter_set_bitC bf ind ind':
+    (bloomfilter_set_bit ind (bloomfilter_set_bit ind' bf)) =
+    (bloomfilter_set_bit ind' (bloomfilter_set_bit ind bf)).
+  Proof.
+    rewrite /bloomfilter_set_bit/bloomfilter_state//.
+    apply f_equal => //.
+    apply eq_from_tnth => pos.
+    case Hpos: (pos == ind); case Hpos': (pos == ind').
+    - by rewrite !FixedList.tnth_set_nth_eq.
+    - rewrite FixedList.tnth_set_nth_eq; last by [].
+      rewrite FixedList.tnth_set_nth_neq; last by move/Bool.negb_true_iff: Hpos' ->.
+        by rewrite FixedList.tnth_set_nth_eq; last by [].
+    - rewrite FixedList.tnth_set_nth_neq; last by move/Bool.negb_true_iff: Hpos ->.
+      rewrite FixedList.tnth_set_nth_eq; last by [].
+        by rewrite FixedList.tnth_set_nth_eq; last by [].
+
+    - rewrite FixedList.tnth_set_nth_neq; last by move/Bool.negb_true_iff: Hpos ->.  
+      rewrite FixedList.tnth_set_nth_neq; last by move/Bool.negb_true_iff: Hpos' ->.
+      rewrite FixedList.tnth_set_nth_neq; last by move/Bool.negb_true_iff: Hpos' ->.  
+        by rewrite FixedList.tnth_set_nth_neq; last by move/Bool.negb_true_iff: Hpos ->.
+  Qed.
+
+
+  Lemma bloomfilter_add_internal_hit bf (ind: 'I_Hash_size.+1) hshs :
+    (ind \in hshs) ->
+    (tnth (bloomfilter_state (bloomfilter_add_internal hshs bf)) ind).
+  Proof.
+    elim: hshs bf  => //= hsh hshs IHs bf.
+
+    rewrite in_cons => /orP [/eqP -> | H]; last by apply IHs.
+
+    clear IHs ind.
+    elim: hshs bf hsh => //.
+    - rewrite /bloomfilter_add_internal/bloomfilter_set_bit/bloomfilter_state //.
+        by move=> bf hsh; rewrite FixedList.tnth_set_nth_eq => //=.
+    - move=> hsh hshs IHs bf hsh'.    
+      move=> //=.
+      rewrite bloomfilter_set_bitC .
+        by apply IHs.
+  Qed.
+
+  Lemma bloomfilter_add_internal_preserve bf ind hshs:
+    tnth (bloomfilter_state bf) ind ->
+    tnth (bloomfilter_state (bloomfilter_add_internal hshs bf)) ind.
+  Proof.
+
+    elim: hshs bf ind => //= hsh hshs IHs bf ind Htnth.
+    apply IHs.
+    rewrite /bloomfilter_set_bit/bloomfilter_state //.
+    case Hhsh: (ind == hsh).
+    - by rewrite FixedList.tnth_set_nth_eq //=.
+    - rewrite FixedList.tnth_set_nth_neq; first by move: Htnth; rewrite/bloomfilter_state//=.
+        by move/Bool.negb_true_iff: Hhsh.
+  Qed.
+
+
+  Lemma bloomfilter_add_internal_miss
+        bf (ind: 'I_Hash_size.+1) hshs :
+    ~~ tnth (bloomfilter_state bf) ind ->
+    ~~ ( ind \in hshs) ->
+    (~~ tnth (bloomfilter_state (bloomfilter_add_internal hshs bf)) ind).
+  Proof.
+
+    move=> Htnth.
+    elim: hshs bf Htnth => //= hsh hshs IHs bf Htnth.
+    move=> H; move: (H).
+    rewrite in_cons.
+    rewrite negb_or => /andP [Hneq Hnotin].
+    apply IHs.
+    rewrite /bloomfilter_state/bloomfilter_set_bit.
+    rewrite FixedList.tnth_set_nth_neq => //=.
+    exact Hnotin.
+  Qed.
+
+
+  Lemma bloomfilter_add_internal_hit_infer bf (ind: 'I_Hash_size.+1) inds:
+    ~~ bloomfilter_get_bit ind bf ->
+    tnth (bloomfilter_state (bloomfilter_add_internal inds bf)) ind ->
+    ind \in inds.
+  Proof.
+    move=> Hbit Htnth.
+    case Hind: (ind \in inds) =>//=; move/Bool.negb_true_iff: Hind => Hind.
+      by move/Bool.negb_true_iff: (bloomfilter_add_internal_miss Hbit Hind) Htnth ->.
+  Qed.
+
+
+  Lemma bloomfilter_set_get_eq hash_value bf :
+    bloomfilter_get_bit hash_value (bloomfilter_set_bit hash_value bf).
+  Proof.
+      by rewrite /bloomfilter_get_bit/bloomfilter_set_bit//
+                 /bloomfilter_state FixedList.tnth_set_nth_eq //=.
+  Qed.
+
+  
+  Lemma bloomfilter_add_insert_contains l (bf: BloomFilter) (inds: l.-tuple 'I_Hash_size.+1 )
+        (ps: seq 'I_Hash_size.+1) :
+    all (fun p => p \in inds) ps -> all (bloomfilter_get_bit^~ (bloomfilter_add_internal inds bf)) ps.
+  Proof.                  
+    move=>/allP HinP; apply/allP => [p Hp].
+      by rewrite /bloomfilter_get_bit/bloomfilter_state bloomfilter_add_internal_hit //=; move: (HinP p Hp).
+  Qed.
+  
+  Lemma bloomfilter_set_bit_conv bf b b':
+    (bloomfilter_set_bit b (bloomfilter_set_bit b' bf)) =
+    (bloomfilter_set_bit b' (bloomfilter_set_bit b bf)).
+  Proof.
+
+    rewrite/bloomfilter_set_bit/bloomfilter_state; apply f_equal.
+    case: bf; rewrite/BitVector=>bf .
+      by rewrite  fixedlist_set_nthC.
+  Qed.
+
+  Lemma bloomfilter_add_multiple_cat bf b others:
+    (bloomfilter_add_internal others (bloomfilter_add_internal b bf)) =
+    (bloomfilter_add_internal (others ++ b) bf).
+  Proof.
+
+    elim: others bf => [//=|other others Hothers] bf //= .
+    rewrite -Hothers; apply f_equal; clear Hothers others.
+    elim: b bf => [//=| b bs Hbs] bf //=.
+    rewrite  bloomfilter_set_bit_conv.
+      by rewrite Hbs.
+  Qed.
+
+  
+  
 End BloomFilter.
